isabelle/Chapter15_2_Typechecking.thy
@@ -6,8 +6,8 @@ inductive typecheck :: "type env => expr => type => bool"
 where tc_var [simp]: "lookup gam x = Some t ==> typecheck gam (Var x) t"
     | tc_zero [simp]: "typecheck gam Zero Nat"
     | tc_suc [simp]: "typecheck gam e Nat ==> typecheck gam (Suc e) Nat"
-    | tc_rec [simp]: "typecheck gam et Nat ==> typecheck gam e0 t ==> 
-                typecheck (extend (extend gam t) Nat) es t ==> typecheck gam (Rec et e0 es) t"
+    | tc_isz [simp]: "typecheck gam et Nat ==> typecheck gam e0 t ==> 
+                typecheck (extend gam Nat) es t ==> typecheck gam (IsZ et e0 es) t"
     | tc_lam [simp]: "typecheck (extend gam t1) e t2 ==> typecheck gam (Lam t1 e) (Arrow t1 t2)"
     | tc_appl [simp]: "typecheck gam e1 (Arrow t2 t) ==> typecheck gam e2 t2 ==> 
                 typecheck gam (Appl e1 e2) t"
@@ -21,11 +21,12 @@ where tc_var [simp]: "lookup gam x = Some t ==> typecheck gam (Var x) t"
                 typecheck (extend gam t2) er t ==> typecheck gam (Case et el er) t"
     | tc_inl [simp]: "typecheck gam e t1 ==> typecheck gam (InL t1 t2 e) (Sum t1 t2)"
     | tc_inr [simp]: "typecheck gam e t2 ==> typecheck gam (InR t1 t2 e) (Sum t1 t2)"
+    | tc_fix [simp]: "typecheck (extend gam t) e t ==> typecheck gam (Fix t e) t"
 
 inductive_cases [elim!]: "typecheck gam (Var x) t"
 inductive_cases [elim!]: "typecheck gam Zero t"
 inductive_cases [elim!]: "typecheck gam (Suc e) t"
-inductive_cases [elim!]: "typecheck gam (Rec et e0 es) t"
+inductive_cases [elim!]: "typecheck gam (IsZ et e0 es) t"
 inductive_cases [elim!]: "typecheck gam (Lam t1 e) t"
 inductive_cases [elim!]: "typecheck gam (Appl e1 e2) t"
 inductive_cases [elim!]: "typecheck gam Triv t"
@@ -36,6 +37,7 @@ inductive_cases [elim!]: "typecheck gam (Abort t1 e) t"
 inductive_cases [elim!]: "typecheck gam (Case et el er) t"
 inductive_cases [elim!]: "typecheck gam (InL t1 t2 e) t"
 inductive_cases [elim!]: "typecheck gam (InR t1 t2 e) t"
+inductive_cases [elim!]: "typecheck gam (Fix t1 e) t"
 
 lemma [simp]: "typecheck gam e t ==> n in gam ==> 
          typecheck (extend_at n gam t') (insert n e) t"
